cogent/llvm/checker/coq/Corres.v
@@ -1,48 +1,45 @@
 From Coq Require Import List String ZArith.
 
-From Checker Require Import Denote Cogent Compiler.
-
 From ITree Require Import ITree ITreeFacts.
 
 From Vellvm Require Import LLVMAst LLVMEvents TopLevel Handlers InterpreterMCFG TopLevelRefinements DynamicTypes
   CFG TypToDtyp InterpretationStack.
 
+From Checker Require Import Denote Cogent Compiler Utils.Fail.
+
 Import ListNotations.
 
 
-Definition vellvm_prog : Type := list (toplevel_entity typ (block typ * list (block typ))).
+Definition vellvm_prog : Type := toplevel_entities typ (block typ * list (block typ)).
 
 (* Lifted from Helix *)
 Definition E_mcfg : Type -> Type := (ExternalCallE +' PickE +' UBE +' DebugE +' FailureE).
-Definition E_cfg : Type -> Type := (CallE +' PickE +' UBE +' DebugE +' FailureE). 
-Definition semantics_llvm_mcfg p : itree E_mcfg _ := model_to_L3 DTYPE_Void "main" main_args p.
-Definition semantics_llvm (prog : list (toplevel_entity typ (LLVMAst.block typ * list (LLVMAst.block typ)))) :=
-  semantics_llvm_mcfg (convert_types (mcfg_of_tle prog)).
+(* Definition E_cfg : Type -> Type := (CallE +' PickE +' UBE +' DebugE +' FailureE).  *)
+Definition semantics_llvm_mcfg p : itree E_mcfg _ := model_to_L3 DTYPE_Void "main" [DV.UVALUE_I32 (DynamicValues.Int32.zero)] p.
+Definition semantics_llvm (p : vellvm_prog) : itree E_mcfg _ :=
+  semantics_llvm_mcfg (convert_types (mcfg_of_tle p)).
 
-Definition vellvm_env : Type := memory_stack * (local_env * global_env).
-Definition interp_vellvm (t : itree L0 uvalue) (e : vellvm_env) : itree L3 res_L3 :=
-  interp_mcfg3 t (snd (snd e)) (fst (snd e), []) (fst e).
+Definition semantics_cogent (p : cogent_prog) : failT (itree E_mcfg) (memory * (locals * uval)) := 
+  interp_cogent (prog_to_module p) (UFunction "main") UUnit empty_locals dummy_memory.
 
-Definition relate_env (c_env : locals) (v_env : vellvm_env) : Prop := True.
+Section TopLevel.
 
-Section Simple.
-
-  (* want to try and relate a CFG to a function *)
-  
+  (* placeholder *)
   Definition TT {A B} (x: A) (y: B):= True.
 
-  Lemma correct :
-    forall
-      (n : name) (t rt : type) (b : expr) 
-      (d : definition typ (block typ * list (block typ))),
-      compile_fun n t rt b = inr d ->
-        eutt TT
-          (interp_cogent (denote_expr b) empty_locals empty_memory) 
-          (interp_cfg2 (denote_cfg (convert_typ [] (cfg_of_definition typ d))) [] []).
+  Lemma compiler_correct :
+    forall (c : cogent_prog) (ll : vellvm_prog),
+      compile_cogent c = inr ll -> eutt TT (semantics_cogent c) (semantics_llvm ll).
   Proof.
   Abort.
 
-End Simple.
+End TopLevel.
+
+(* Definition vellvm_env : Type := memory_stack * (local_env * global_env).
+Definition interp_vellvm (t : itree L0 uvalue) (e : vellvm_env) : itree L3 res_L3 :=
+  interp_mcfg3 t (snd (snd e)) (fst (snd e), []) (fst e).
+
+Definition relate_env (c_env : locals) (v_env : vellvm_env) : Prop := True. *)
 
 (* Section RAB.
 
